Cslib/Logics/Modal/Metalogic/Systems/S4/Completeness.lean
@@ -8,7 +8,6 @@ module
 
 
 public import Cslib.Logics.Modal.Metalogic.Completeness
-public import Cslib.Logics.Modal.Metalogic.StrongCompleteness
 public import Cslib.Logics.Modal.Metalogic.Systems.S4.Soundness
 public import Cslib.Logics.Modal.ProofSystem.Instances
 
